WP rules for Jmp, Jnz and Jalr

theories/rules/rules_Jnz.v
@@ -17,34 +17,50 @@ Section cap_lang_rules.
   Implicit Types reg : gmap RegName Word.
   Implicit Types ms : gmap Addr Word.
 
-  Inductive Jnz_spec (regs: Reg) (dst src: RegName) : Reg → cap_lang.val → Prop :=
-  | Jnz_spec_failure w:
-      regs !! src = Some w →
-      nonZero w = false →
+  Inductive Jnz_failure (regs: Reg) (rimm: Z + RegName) (rcond : RegName) :=
+  | Jnz_fail_PC_overflow_next cond:
+      regs !! rcond = Some cond →
+      nonZero cond = false →
       incrementPC regs = None →
-      Jnz_spec regs dst src regs FailedV
-  | Jnz_spec_success1 w regs':
-      regs !! src = Some w →
-      nonZero w = false →
-      incrementPC regs = Some regs' →
-      Jnz_spec regs dst src regs' NextIV
-  | Jnz_spec_success2 w w':
-      regs !! src = Some w →
-      regs !! dst = Some w' →
-      nonZero w = true →
-      Jnz_spec regs dst src (<[PC := updatePcPerm w' ]> regs) NextIV.
+      Jnz_failure regs rimm rcond
+  | Jnz_fail_PC_overflow_jmp imm cond:
+      regs !! rcond = Some cond →
+      nonZero cond = true →
+      incrementPC_gen regs imm = None →
+      Jnz_failure regs rimm rcond
+  | Jnz_fail_no_imm cond:
+      regs !! rcond = Some cond →
+      nonZero cond = true →
+      z_of_argument regs rimm = None →
+      Jnz_failure regs rimm rcond.
 
-  Lemma wp_Jnz Ep pc_p pc_g pc_b pc_e pc_a w dst src regs :
-    decodeInstrW w = Jnz dst src ->
+  Inductive Jnz_spec (regs: Reg) (rimm: Z + RegName) (rcond : RegName) : Reg → cap_lang.val → Prop :=
+  | Jnz_spec_success_next regs' cond :
+      regs !! rcond = Some cond →
+      nonZero cond = false →
+      incrementPC regs = Some regs' →
+      Jnz_spec regs rimm rcond regs' NextIV
+  | Jnz_spec_success_jmp regs' imm cond :
+      regs !! rcond = Some cond →
+      nonZero cond = true →
+      z_of_argument regs rimm = Some imm →
+      incrementPC_gen regs imm = Some regs' →
+      Jnz_spec regs rimm rcond regs' NextIV
+  | Jnz_spec_failure:
+      Jnz_failure regs rimm rcond →
+      Jnz_spec regs rimm rcond regs FailedV.
+
+  Lemma wp_Jnz Ep pc_p pc_g pc_b pc_e pc_a w rimm rcond regs :
+    decodeInstrW w = Jnz rimm rcond ->
     isCorrectPC (WCap pc_p pc_g pc_b pc_e pc_a) →
     regs !! PC = Some (WCap pc_p pc_g pc_b pc_e pc_a) →
-    regs_of (Jnz dst src) ⊆ dom regs →
+    regs_of (Jnz rimm rcond) ⊆ dom regs →
 
     {{{ ▷ pc_a ↦ₐ w ∗
         ▷ [∗ map] k↦y ∈ regs, k ↦ᵣ y }}}
       Instr Executable @ Ep
     {{{ regs' retv, RET retv;
-        ⌜ Jnz_spec regs dst src regs' retv ⌝ ∗
+        ⌜ Jnz_spec regs rimm rcond regs' retv ⌝ ∗
         pc_a ↦ₐ w ∗
         [∗ map] k↦y ∈ regs', k ↦ᵣ y }}}.
   Proof.
@@ -62,199 +78,232 @@ Section cap_lang_rules.
 
     specialize (indom_regs_incl _ _ _ Dregs Hregs) as Hri.
     unfold regs_of in Hri, Dregs.
-    destruct (Hri src) as [wsrc [H'src Hsrc]]. by set_solver+.
-    destruct (Hri dst) as [wdst [H'dst Hdst]]. by set_solver+.
+    destruct (Hri rcond) as [wrcond [H'rcond Hrcond]]; first by set_solver+.
     unfold exec in Hstep; cbn in Hstep.
+    rewrite Hrcond /= in Hstep.
 
-    destruct (nonZero wsrc) eqn:Hnz; pose proof Hnz as H'nz;
-      cbn in Hstep; rewrite Hsrc Hdst /= Hnz in Hstep.
-    { inv Hstep. simplify_pair_eq.
+    destruct (nonZero wrcond) eqn:Hnz; pose proof Hnz as H'nz; cbn in Hstep.
+    - destruct (z_of_argument regs rimm) as [imm|] eqn:Himm
+      ; pose proof Himm as H'imm
+      ; cycle 1.
+      { (* Failure: argument is not a constant (z_of_argument regs arg = None) *)
+        unfold z_of_argument in Himm, Hstep.
+        destruct rimm as [| rimm]; [ congruence |].
+        odestruct (Hri rimm) as [rimmv [Hrimm' Hrimm]].
+        { unfold regs_of_argument. set_solver+. }
+        rewrite Hrimm Hrimm' in Himm Hstep.
+        assert (c = Failed ∧ σ2 = (r, sr, m)) as (-> & ->).
+        { destruct_word rimmv; cbn in Hstep; try congruence; by simplify_pair_eq. }
+        iFailWP "Hφ" Jnz_fail_no_imm. }
+      apply (z_of_arg_mono _ r) in Himm; auto.
+      rewrite Himm in Hstep; simpl in Hstep.
+
+      destruct (incrementPC_gen regs imm) eqn:Hregs';
+        pose proof Hregs' as H'regs'; cycle 1.
+      {
+        assert (incrementPC_gen r imm = None) as HH.
+        { eapply incrementPC_gen_overflow_mono; first eapply Hregs' ; eauto. }
+        apply (incrementPC_gen_fail_updatePC_gen _ sr m) in HH. rewrite HH in Hstep.
+        assert (c = Failed ∧ σ2 = (r, sr, m)) as (-> & ->) by (inversion Hstep; auto).
+        iFailWP "Hφ" Jnz_fail_PC_overflow_jmp. }
+
+      eapply (incrementPC_gen_success_updatePC_gen _ sr m _ imm) in Hregs'
+          as (p'' & g'' & b' & e' & a'' & a''' & a_pc' & HPC'' & HuPC & ->).
+      eapply updatePC_gen_success_incl with (sregs':=sr) (m':=m) in HuPC; eauto.
+      rewrite HuPC in Hstep.
+      eassert ((c, σ2) = (NextI, _)) as HH.
+      { cbn in *; eauto. }
+      simplify_pair_eq.
+
       iMod ((gen_heap_update_inSepM _ _ PC) with "Hr Hmap") as "[Hr Hmap]"; eauto.
-      iFrame. iApply "Hφ". iFrame. iPureIntro. econstructor 3; eauto. }
+      iFrame.
+      iApply "Hφ". iFrame. iPureIntro.
+      eapply Jnz_spec_success_jmp; eauto.
+    - destruct (incrementPC regs) eqn:HX; pose proof HX as H'X; cycle 1.
+      { apply incrementPC_fail_updatePC with (sregs:=sr) (m:=m) in HX.
+        eapply updatePC_fail_incl with (sregs':=sr) (m':=m) in HX; eauto.
+        rewrite HX in Hstep. inv Hstep.
+        iFailWP "Hφ" Jnz_fail_PC_overflow_next. }
 
-    destruct (incrementPC regs) eqn:HX; pose proof HX as H'X; cycle 1.
-    { apply incrementPC_fail_updatePC with (sregs:=sr) (m:=m) in HX.
-      eapply updatePC_fail_incl with (sregs':=sr) (m':=m) in HX; eauto.
-      rewrite HX in Hstep. inv Hstep.
-      iFrame. iApply "Hφ". iFrame. iPureIntro; econstructor; eauto. }
-
-    destruct (incrementPC_success_updatePC _ sr m _ HX)
-      as (p' & g' & b' & e' & a'' & a''' & a_pc' & HPC'' & HuPC & ->).
-    eapply updatePC_success_incl with (sregs':=sr) (m':=m) in HuPC; eauto. rewrite HuPC in Hstep.
-    simplify_pair_eq.
-    iMod ((gen_heap_update_inSepM _ _ PC) with "Hr Hmap") as "[Hr Hmap]"; eauto.
-    iFrame. iApply "Hφ". iFrame. iPureIntro. econstructor 2; eauto.
+      destruct (incrementPC_success_updatePC _ sr m _ HX)
+        as (p' & g' & b' & e' & a'' & a''' & a_pc' & HPC'' & HuPC & ->).
+      eapply updatePC_success_incl with (sregs':=sr) (m':=m) in HuPC; eauto. rewrite HuPC in Hstep.
+      simplify_pair_eq.
+      iMod ((gen_heap_update_inSepM _ _ PC) with "Hr Hmap") as "[Hr Hmap]"; eauto.
+      iFrame. iApply "Hφ". iFrame. iPureIntro.
+      eapply Jnz_spec_success_next; eauto.
   Qed.
 
-  Lemma wp_jnz_success_jmp E r1 r2 pc_p pc_g pc_b pc_e pc_a w w1 w2 :
-    decodeInstrW w = Jnz r1 r2 →
-    isCorrectPC (WCap pc_p pc_g pc_b pc_e pc_a) →
-    w2 ≠ WInt 0%Z →
+  (* TODO fix the instantiated rules *)
+  (* Lemma wp_jnz_success_jmp E r1 r2 pc_p pc_g pc_b pc_e pc_a w w1 w2 : *)
+  (*   decodeInstrW w = Jnz r1 r2 → *)
+  (*   isCorrectPC (WCap pc_p pc_g pc_b pc_e pc_a) → *)
+  (*   w2 ≠ WInt 0%Z → *)
 
-    {{{ ▷ PC ↦ᵣ WCap pc_p pc_g pc_b pc_e pc_a
-        ∗ ▷ pc_a ↦ₐ w
-        ∗ ▷ r1 ↦ᵣ w1
-        ∗ ▷ r2 ↦ᵣ w2 }}}
-      Instr Executable @ E
-      {{{ RET NextIV;
-          PC ↦ᵣ updatePcPerm w1
-          ∗ pc_a ↦ₐ w
-          ∗ r1 ↦ᵣ w1
-          ∗ r2 ↦ᵣ w2 }}}.
-  Proof.
-    iIntros (Hinstr Hvpc Hne ϕ) "(>HPC & >Hpc_a & >Hr1 & >Hr2) Hφ".
-    iDestruct (map_of_regs_3 with "HPC Hr1 Hr2") as "[Hmap (%&%&%)]".
-    iApply (wp_Jnz with "[$Hmap Hpc_a]"); eauto; simplify_map_eq; eauto.
-    by unfold regs_of; rewrite !dom_insert; set_solver+.
-    iNext. iIntros (regs' retv) "(#Hspec & Hpc_a & Hmap)". iDestruct "Hspec" as %Hspec.
+  (*   {{{ ▷ PC ↦ᵣ WCap pc_p pc_g pc_b pc_e pc_a *)
+  (*       ∗ ▷ pc_a ↦ₐ w *)
+  (*       ∗ ▷ r1 ↦ᵣ w1 *)
+  (*       ∗ ▷ r2 ↦ᵣ w2 }}} *)
+  (*     Instr Executable @ E *)
+  (*     {{{ RET NextIV; *)
+  (*         PC ↦ᵣ updatePcPerm w1 *)
+  (*         ∗ pc_a ↦ₐ w *)
+  (*         ∗ r1 ↦ᵣ w1 *)
+  (*         ∗ r2 ↦ᵣ w2 }}}. *)
+  (* Proof. *)
+  (*   iIntros (Hinstr Hvpc Hne ϕ) "(>HPC & >Hpc_a & >Hr1 & >Hr2) Hφ". *)
+  (*   iDestruct (map_of_regs_3 with "HPC Hr1 Hr2") as "[Hmap (%&%&%)]". *)
+  (*   iApply (wp_Jnz with "[$Hmap Hpc_a]"); eauto; simplify_map_eq; eauto. *)
+  (*   by unfold regs_of; rewrite !dom_insert; set_solver+. *)
+  (*   iNext. iIntros (regs' retv) "(#Hspec & Hpc_a & Hmap)". iDestruct "Hspec" as %Hspec. *)
 
-    assert (nonZero w2 = true).
-    { unfold nonZero, Zneq_bool in *.
-      repeat case_match; try congruence; subst. exfalso.
-      apply Hne. f_equal. by apply Z.compare_eq. }
+  (*   assert (nonZero w2 = true). *)
+  (*   { unfold nonZero, Zneq_bool in *. *)
+  (*     repeat case_match; try congruence; subst. exfalso. *)
+  (*     apply Hne. f_equal. by apply Z.compare_eq. } *)
 
-   destruct Hspec as [ | | ].
-   { exfalso. simplify_map_eq. congruence. }
-   { exfalso. simplify_map_eq. congruence. }
-   { iApply "Hφ". iFrame. simplify_map_eq. rewrite insert_insert.
-     iDestruct (regs_of_map_3 with "Hmap") as "(?&?&?)"; eauto; iFrame. }
-  Qed.
+  (*  destruct Hspec as [ | | ]. *)
+  (*  { exfalso. simplify_map_eq. congruence. } *)
+  (*  { exfalso. simplify_map_eq. congruence. } *)
+  (*  { iApply "Hφ". iFrame. simplify_map_eq. rewrite insert_insert. *)
+  (*    iDestruct (regs_of_map_3 with "Hmap") as "(?&?&?)"; eauto; iFrame. } *)
+  (* Qed. *)
 
-  Lemma wp_jnz_success_jmp2 E r2 pc_p pc_g pc_b pc_e pc_a w w2 :
-    decodeInstrW w = Jnz r2 r2 →
-    isCorrectPC (WCap pc_p pc_g pc_b pc_e pc_a) →
-    w2 ≠ WInt 0%Z →
+  (* Lemma wp_jnz_success_jmp2 E r2 pc_p pc_g pc_b pc_e pc_a w w2 : *)
+  (*   decodeInstrW w = Jnz r2 r2 → *)
+  (*   isCorrectPC (WCap pc_p pc_g pc_b pc_e pc_a) → *)
+  (*   w2 ≠ WInt 0%Z → *)
 
-    {{{ ▷ PC ↦ᵣ WCap pc_p pc_g pc_b pc_e pc_a
-        ∗ ▷ pc_a ↦ₐ w
-        ∗ ▷ r2 ↦ᵣ w2 }}}
-      Instr Executable @ E
-      {{{ RET NextIV;
-          PC ↦ᵣ updatePcPerm w2
-          ∗ pc_a ↦ₐ w
-          ∗ r2 ↦ᵣ w2 }}}.
-  Proof.
-    iIntros (Hinstr Hvpc Hne ϕ) "(>HPC & >Hpc_a & >Hr2) Hφ".
-    iDestruct (map_of_regs_2 with "HPC Hr2") as "[Hmap %]".
-    iApply (wp_Jnz with "[$Hmap Hpc_a]"); eauto; simplify_map_eq; eauto.
-    by unfold regs_of; rewrite !dom_insert; set_solver+.
-    iNext. iIntros (regs' retv) "(#Hspec & Hpc_a & Hmap)". iDestruct "Hspec" as %Hspec.
+  (*   {{{ ▷ PC ↦ᵣ WCap pc_p pc_g pc_b pc_e pc_a *)
+  (*       ∗ ▷ pc_a ↦ₐ w *)
+  (*       ∗ ▷ r2 ↦ᵣ w2 }}} *)
+  (*     Instr Executable @ E *)
+  (*     {{{ RET NextIV; *)
+  (*         PC ↦ᵣ updatePcPerm w2 *)
+  (*         ∗ pc_a ↦ₐ w *)
+  (*         ∗ r2 ↦ᵣ w2 }}}. *)
+  (* Proof. *)
+  (*   iIntros (Hinstr Hvpc Hne ϕ) "(>HPC & >Hpc_a & >Hr2) Hφ". *)
+  (*   iDestruct (map_of_regs_2 with "HPC Hr2") as "[Hmap %]". *)
+  (*   iApply (wp_Jnz with "[$Hmap Hpc_a]"); eauto; simplify_map_eq; eauto. *)
+  (*   by unfold regs_of; rewrite !dom_insert; set_solver+. *)
+  (*   iNext. iIntros (regs' retv) "(#Hspec & Hpc_a & Hmap)". iDestruct "Hspec" as %Hspec. *)
 
-    assert (nonZero w2 = true).
-    { unfold nonZero, Zneq_bool in *.
-      repeat case_match; try congruence; subst. exfalso.
-      apply Hne. f_equal. by apply Z.compare_eq. }
+  (*   assert (nonZero w2 = true). *)
+  (*   { unfold nonZero, Zneq_bool in *. *)
+  (*     repeat case_match; try congruence; subst. exfalso. *)
+  (*     apply Hne. f_equal. by apply Z.compare_eq. } *)
 
-   destruct Hspec as [ | | ].
-   { exfalso. simplify_map_eq. congruence. }
-   { exfalso. simplify_map_eq. congruence. }
-   { iApply "Hφ". iFrame. simplify_map_eq. rewrite insert_insert.
-     iDestruct (regs_of_map_2 with "Hmap") as "(?&?)"; eauto; iFrame. }
-  Qed.
+  (*  destruct Hspec as [ | | ]. *)
+  (*  { exfalso. simplify_map_eq. congruence. } *)
+  (*  { exfalso. simplify_map_eq. congruence. } *)
+  (*  { iApply "Hφ". iFrame. simplify_map_eq. rewrite insert_insert. *)
+  (*    iDestruct (regs_of_map_2 with "Hmap") as "(?&?)"; eauto; iFrame. } *)
+  (* Qed. *)
 
-  Lemma wp_jnz_success_jmpPC E pc_p pc_g pc_b pc_e pc_a w :
-    decodeInstrW w = Jnz PC PC →
-    isCorrectPC (WCap pc_p pc_g pc_b pc_e pc_a) →
+  (* Lemma wp_jnz_success_jmpPC E pc_p pc_g pc_b pc_e pc_a w : *)
+  (*   decodeInstrW w = Jnz PC PC → *)
+  (*   isCorrectPC (WCap pc_p pc_g pc_b pc_e pc_a) → *)
 
-    {{{ ▷ PC ↦ᵣ WCap pc_p pc_g pc_b pc_e pc_a
-        ∗ ▷ pc_a ↦ₐ w }}}
-      Instr Executable @ E
-      {{{ RET NextIV;
-          PC ↦ᵣ updatePcPerm (WCap pc_p pc_g pc_b pc_e pc_a)
-          ∗ pc_a ↦ₐ w }}}.
-  Proof.
-    iIntros (Hinstr Hvpc ϕ) "(>HPC & >Hpc_a) Hφ".
-    iDestruct (map_of_regs_1 with "HPC") as "Hmap".
-    iApply (wp_Jnz with "[$Hmap Hpc_a]"); eauto; simplify_map_eq; eauto.
-    iNext. iIntros (regs' retv) "(#Hspec & Hpc_a & Hmap)". iDestruct "Hspec" as %Hspec.
+  (*   {{{ ▷ PC ↦ᵣ WCap pc_p pc_g pc_b pc_e pc_a *)
+  (*       ∗ ▷ pc_a ↦ₐ w }}} *)
+  (*     Instr Executable @ E *)
+  (*     {{{ RET NextIV; *)
+  (*         PC ↦ᵣ updatePcPerm (WCap pc_p pc_g pc_b pc_e pc_a) *)
+  (*         ∗ pc_a ↦ₐ w }}}. *)
+  (* Proof. *)
+  (*   iIntros (Hinstr Hvpc ϕ) "(>HPC & >Hpc_a) Hφ". *)
+  (*   iDestruct (map_of_regs_1 with "HPC") as "Hmap". *)
+  (*   iApply (wp_Jnz with "[$Hmap Hpc_a]"); eauto; simplify_map_eq; eauto. *)
+  (*   iNext. iIntros (regs' retv) "(#Hspec & Hpc_a & Hmap)". iDestruct "Hspec" as %Hspec. *)
 
-   destruct Hspec as [ | | ]; [ by simplify_map_eq .. | ].
-   { iApply "Hφ". iFrame. simplify_map_eq. rewrite insert_insert.
-     iDestruct (regs_of_map_1 with "Hmap") as "?"; eauto; iFrame. }
-  Qed.
+  (*  destruct Hspec as [ | | ]; [ by simplify_map_eq .. | ]. *)
+  (*  { iApply "Hφ". iFrame. simplify_map_eq. rewrite insert_insert. *)
+  (*    iDestruct (regs_of_map_1 with "Hmap") as "?"; eauto; iFrame. } *)
+  (* Qed. *)
 
-  Lemma wp_jnz_success_jmpPC1 E r2 pc_p pc_g pc_b pc_e pc_a w w2 :
-    decodeInstrW w = Jnz PC r2 →
-    isCorrectPC (WCap pc_p pc_g pc_b pc_e pc_a) →
-    w2 ≠ WInt 0%Z →
+  (* Lemma wp_jnz_success_jmpPC1 E r2 pc_p pc_g pc_b pc_e pc_a w w2 : *)
+  (*   decodeInstrW w = Jnz PC r2 → *)
+  (*   isCorrectPC (WCap pc_p pc_g pc_b pc_e pc_a) → *)
+  (*   w2 ≠ WInt 0%Z → *)
 
-    {{{ ▷ PC ↦ᵣ WCap pc_p pc_g pc_b pc_e pc_a
-        ∗ ▷ pc_a ↦ₐ w
-        ∗ ▷ r2 ↦ᵣ w2 }}}
-      Instr Executable @ E
-      {{{ RET NextIV;
-          PC ↦ᵣ updatePcPerm (WCap pc_p pc_g pc_b pc_e pc_a)
-          ∗ pc_a ↦ₐ w
-          ∗ r2 ↦ᵣ w2 }}}.
-  Proof.
-    iIntros (Hinstr Hvpc Hne ϕ) "(>HPC & >Hpc_a & >Hr2) Hφ".
-    iDestruct (map_of_regs_2 with "HPC Hr2") as "[Hmap %]".
-    iApply (wp_Jnz with "[$Hmap Hpc_a]"); eauto; simplify_map_eq; eauto.
-    by unfold regs_of; rewrite !dom_insert; set_solver+.
-    iNext. iIntros (regs' retv) "(#Hspec & Hpc_a & Hmap)". iDestruct "Hspec" as %Hspec.
+  (*   {{{ ▷ PC ↦ᵣ WCap pc_p pc_g pc_b pc_e pc_a *)
+  (*       ∗ ▷ pc_a ↦ₐ w *)
+  (*       ∗ ▷ r2 ↦ᵣ w2 }}} *)
+  (*     Instr Executable @ E *)
+  (*     {{{ RET NextIV; *)
+  (*         PC ↦ᵣ updatePcPerm (WCap pc_p pc_g pc_b pc_e pc_a) *)
+  (*         ∗ pc_a ↦ₐ w *)
+  (*         ∗ r2 ↦ᵣ w2 }}}. *)
+  (* Proof. *)
+  (*   iIntros (Hinstr Hvpc Hne ϕ) "(>HPC & >Hpc_a & >Hr2) Hφ". *)
+  (*   iDestruct (map_of_regs_2 with "HPC Hr2") as "[Hmap %]". *)
+  (*   iApply (wp_Jnz with "[$Hmap Hpc_a]"); eauto; simplify_map_eq; eauto. *)
+  (*   by unfold regs_of; rewrite !dom_insert; set_solver+. *)
+  (*   iNext. iIntros (regs' retv) "(#Hspec & Hpc_a & Hmap)". iDestruct "Hspec" as %Hspec. *)
 
-    assert (nonZero w2 = true).
-    { unfold nonZero, Zneq_bool in *.
-      repeat case_match; try congruence; subst. exfalso.
-      apply Hne. f_equal. by apply Z.compare_eq. }
+  (*   assert (nonZero w2 = true). *)
+  (*   { unfold nonZero, Zneq_bool in *. *)
+  (*     repeat case_match; try congruence; subst. exfalso. *)
+  (*     apply Hne. f_equal. by apply Z.compare_eq. } *)
 
-   destruct Hspec as [ | | ].
-   { exfalso. simplify_map_eq. congruence. }
-   { exfalso. simplify_map_eq. congruence. }
-   { iApply "Hφ". iFrame. simplify_map_eq. rewrite insert_insert.
-     iDestruct (regs_of_map_2 with "Hmap") as "(?&?)"; eauto; iFrame. }
-  Qed.
+  (*  destruct Hspec as [ | | ]. *)
+  (*  { exfalso. simplify_map_eq. congruence. } *)
+  (*  { exfalso. simplify_map_eq. congruence. } *)
+  (*  { iApply "Hφ". iFrame. simplify_map_eq. rewrite insert_insert. *)
+  (*    iDestruct (regs_of_map_2 with "Hmap") as "(?&?)"; eauto; iFrame. } *)
+  (* Qed. *)
 
-  Lemma wp_jnz_success_jmpPC2 E r1 pc_p pc_g pc_b pc_e pc_a w w1 :
-    decodeInstrW w = Jnz r1 PC →
-    isCorrectPC (WCap pc_p pc_g pc_b pc_e pc_a) →
+  (* Lemma wp_jnz_success_jmpPC2 E r1 pc_p pc_g pc_b pc_e pc_a w w1 : *)
+  (*   decodeInstrW w = Jnz r1 PC → *)
+  (*   isCorrectPC (WCap pc_p pc_g pc_b pc_e pc_a) → *)
 
-    {{{ ▷ PC ↦ᵣ WCap pc_p pc_g pc_b pc_e pc_a
-        ∗ ▷ pc_a ↦ₐ w
-        ∗ ▷ r1 ↦ᵣ w1 }}}
-      Instr Executable @ E
-      {{{ RET NextIV;
-          PC ↦ᵣ updatePcPerm w1
-          ∗ pc_a ↦ₐ w
-          ∗ r1 ↦ᵣ w1 }}}.
-  Proof.
-    iIntros (Hinstr Hvpc ϕ) "(>HPC & >Hpc_a & >Hr1) Hφ".
-    iDestruct (map_of_regs_2 with "HPC Hr1") as "[Hmap %]".
-    iApply (wp_Jnz with "[$Hmap Hpc_a]"); eauto; simplify_map_eq; eauto.
-    by unfold regs_of; rewrite !dom_insert; set_solver+.
-    iNext. iIntros (regs' retv) "(#Hspec & Hpc_a & Hmap)". iDestruct "Hspec" as %Hspec.
+  (*   {{{ ▷ PC ↦ᵣ WCap pc_p pc_g pc_b pc_e pc_a *)
+  (*       ∗ ▷ pc_a ↦ₐ w *)
+  (*       ∗ ▷ r1 ↦ᵣ w1 }}} *)
+  (*     Instr Executable @ E *)
+  (*     {{{ RET NextIV; *)
+  (*         PC ↦ᵣ updatePcPerm w1 *)
+  (*         ∗ pc_a ↦ₐ w *)
+  (*         ∗ r1 ↦ᵣ w1 }}}. *)
+  (* Proof. *)
+  (*   iIntros (Hinstr Hvpc ϕ) "(>HPC & >Hpc_a & >Hr1) Hφ". *)
+  (*   iDestruct (map_of_regs_2 with "HPC Hr1") as "[Hmap %]". *)
+  (*   iApply (wp_Jnz with "[$Hmap Hpc_a]"); eauto; simplify_map_eq; eauto. *)
+  (*   by unfold regs_of; rewrite !dom_insert; set_solver+. *)
+  (*   iNext. iIntros (regs' retv) "(#Hspec & Hpc_a & Hmap)". iDestruct "Hspec" as %Hspec. *)
 
-   destruct Hspec as [ | | ]; [ by simplify_map_eq .. | ].
-   { iApply "Hφ". iFrame. simplify_map_eq. rewrite insert_insert.
-     iDestruct (regs_of_map_2 with "Hmap") as "(?&?)"; eauto; iFrame. }
-  Qed.
+  (*  destruct Hspec as [ | | ]; [ by simplify_map_eq .. | ]. *)
+  (*  { iApply "Hφ". iFrame. simplify_map_eq. rewrite insert_insert. *)
+  (*    iDestruct (regs_of_map_2 with "Hmap") as "(?&?)"; eauto; iFrame. } *)
+  (* Qed. *)
 
-  Lemma wp_jnz_success_next E r1 r2 pc_p pc_g pc_b pc_e pc_a pc_a' w w1 :
-    decodeInstrW w = Jnz r1 r2 →
-    isCorrectPC (WCap pc_p pc_g pc_b pc_e pc_a) →
-    (pc_a + 1)%a = Some pc_a' →
+  (* Lemma wp_jnz_success_next E r1 r2 pc_p pc_g pc_b pc_e pc_a pc_a' w w1 : *)
+  (*   decodeInstrW w = Jnz r1 r2 → *)
+  (*   isCorrectPC (WCap pc_p pc_g pc_b pc_e pc_a) → *)
+  (*   (pc_a + 1)%a = Some pc_a' → *)
 
-    {{{ ▷ PC ↦ᵣ WCap pc_p pc_g pc_b pc_e pc_a
-        ∗ ▷ pc_a ↦ₐ w
-        ∗ ▷ r1 ↦ᵣ w1
-        ∗ ▷ r2 ↦ᵣ WInt 0%Z }}}
-      Instr Executable @ E
-      {{{ RET NextIV;
-          PC ↦ᵣ WCap pc_p pc_g pc_b pc_e pc_a'
-          ∗ pc_a ↦ₐ w
-          ∗ r1 ↦ᵣ w1
-          ∗ r2 ↦ᵣ WInt 0%Z }}}.
-  Proof.
-    iIntros (Hinstr Hvpc Hpc_a' ϕ) "(>HPC & >Hpc_a & >Hr1 & >Hr2) Hφ".
-    iDestruct (map_of_regs_3 with "HPC Hr1 Hr2") as "[Hmap (%&%&%)]".
-    iApply (wp_Jnz with "[$Hmap Hpc_a]"); eauto; simplify_map_eq; eauto.
-    by unfold regs_of; rewrite !dom_insert; set_solver+.
-    iNext. iIntros (regs' retv) "(#Hspec & Hpc_a & Hmap)". iDestruct "Hspec" as %Hspec.
+  (*   {{{ ▷ PC ↦ᵣ WCap pc_p pc_g pc_b pc_e pc_a *)
+  (*       ∗ ▷ pc_a ↦ₐ w *)
+  (*       ∗ ▷ r1 ↦ᵣ w1 *)
+  (*       ∗ ▷ r2 ↦ᵣ WInt 0%Z }}} *)
+  (*     Instr Executable @ E *)
+  (*     {{{ RET NextIV; *)
+  (*         PC ↦ᵣ WCap pc_p pc_g pc_b pc_e pc_a' *)
+  (*         ∗ pc_a ↦ₐ w *)
+  (*         ∗ r1 ↦ᵣ w1 *)
+  (*         ∗ r2 ↦ᵣ WInt 0%Z }}}. *)
+  (* Proof. *)
+  (*   iIntros (Hinstr Hvpc Hpc_a' ϕ) "(>HPC & >Hpc_a & >Hr1 & >Hr2) Hφ". *)
+  (*   iDestruct (map_of_regs_3 with "HPC Hr1 Hr2") as "[Hmap (%&%&%)]". *)
+  (*   iApply (wp_Jnz with "[$Hmap Hpc_a]"); eauto; simplify_map_eq; eauto. *)
+  (*   by unfold regs_of; rewrite !dom_insert; set_solver+. *)
+  (*   iNext. iIntros (regs' retv) "(#Hspec & Hpc_a & Hmap)". iDestruct "Hspec" as %Hspec. *)
 
-   destruct Hspec as [ | | ]; try incrementPC_inv; simplify_map_eq; eauto.
-   { congruence. }
-   { iApply "Hφ". iFrame. rewrite insert_insert.
-     iDestruct (regs_of_map_3 with "Hmap") as "(?&?&?)"; eauto; iFrame. }
-  Qed.
+  (*  destruct Hspec as [ | | ]; try incrementPC_inv; simplify_map_eq; eauto. *)
+  (*  { congruence. } *)
+  (*  { iApply "Hφ". iFrame. rewrite insert_insert. *)
+  (*    iDestruct (regs_of_map_3 with "Hmap") as "(?&?&?)"; eauto; iFrame. } *)
+  (* Qed. *)
 
 End cap_lang_rules.
