theories/rules/rules_Jalr.v
@@ -1,0 +1,134 @@
+From iris.base_logic Require Export invariants gen_heap.
+From iris.program_logic Require Export weakestpre ectx_lifting.
+From iris.proofmode Require Import proofmode.
+From iris.algebra Require Import frac.
+From cap_machine Require Export rules_base.
+
+Section cap_lang_rules.
+  Context `{MP: MachineParameters}.
+  Context `{ceriseg: ceriseG Σ}.
+  Implicit Types P Q : iProp Σ.
+  Implicit Types σ : ExecConf.
+  Implicit Types c : cap_lang.expr.
+  Implicit Types a b : Addr.
+  Implicit Types r : RegName.
+  Implicit Types v : cap_lang.val.
+  Implicit Types w : Word.
+  Implicit Types reg : gmap RegName Word.
+  Implicit Types ms : gmap Addr Word.
+
+  Lemma wp_jalr_success E pc_p pc_g pc_b pc_e pc_a pc_a' w rdst wdst wra :
+    decodeInstrW w = Jalr rdst →
+    isCorrectPC (WCap pc_p pc_g pc_b pc_e pc_a) →
+    (pc_a + 1)%a = Some pc_a' →
+
+    {{{ ▷ PC ↦ᵣ WCap pc_p pc_g pc_b pc_e pc_a
+        ∗ ▷ pc_a ↦ₐ w
+        ∗ ▷ rdst ↦ᵣ wdst
+        ∗ ▷ cra ↦ᵣ wra
+    }}}
+      Instr Executable @ E
+      {{{ RET NextIV;
+          PC ↦ᵣ updatePcPerm wdst
+          ∗ pc_a ↦ₐ w
+          ∗ rdst ↦ᵣ wdst
+          ∗ cra ↦ᵣ WCap (seal_perm_sentry pc_p) pc_g pc_b pc_e pc_a'
+      }}}.
+  Proof.
+    iIntros (Hinstr Hvpc Hpca' ϕ) "(>HPC & >Hpc_a & >Hrdst & >Hcra) Hφ".
+    iApply wp_lift_atomic_base_step_no_fork; auto.
+    iIntros (σ1 ns l1 l2 nt) "[ [Hr0 Hsr] Hm ] /=". destruct σ1 as [ [r0 sr] m]; cbn.
+    iDestruct (@gen_heap_valid with "Hm Hpc_a") as %?; auto.
+    iDestruct (@gen_heap_valid with "Hr0 HPC") as %?.
+    iDestruct (@gen_heap_valid with "Hr0 Hrdst") as %Hr_rdst.
+    iDestruct (@gen_heap_valid with "Hr0 Hcra") as %Hr_cra.
+    iModIntro. iSplitR. by iPureIntro; apply normal_always_base_reducible.
+    iNext. iIntros (e2 σ2 efs Hpstep).
+    apply prim_step_exec_inv in Hpstep as (-> & -> & (c & -> & Hstep)).
+    iIntros "_".
+    iSplitR; auto. eapply step_exec_inv in Hstep; eauto.
+    unfold exec, exec_opt in Hstep.
+    rewrite Hr_rdst //= H0 //= Hpca' in Hstep.
+    simplify_pair_eq.
+
+    iMod (@gen_heap_update with "Hr0 Hcra") as "[Hr0 Hcra]".
+    iMod (@gen_heap_update with "Hr0 HPC") as "[Hr0 HPC]".
+    iFrame.
+    iApply "Hφ". by iFrame.
+  Qed.
+
+  Lemma wp_jalr_successPC E pc_p pc_g pc_b pc_e pc_a pc_a' w wra :
+    decodeInstrW w = Jalr PC →
+    isCorrectPC (WCap pc_p pc_g pc_b pc_e pc_a) →
+    (pc_a + 1)%a = Some pc_a' →
+
+    {{{ ▷ PC ↦ᵣ WCap pc_p pc_g pc_b pc_e pc_a
+        ∗ ▷ pc_a ↦ₐ w
+        ∗ ▷ cra ↦ᵣ wra
+    }}}
+      Instr Executable @ E
+      {{{ RET NextIV;
+          PC ↦ᵣ updatePcPerm (WCap pc_p pc_g pc_b pc_e pc_a)
+          ∗ pc_a ↦ₐ w
+          ∗ cra ↦ᵣ WCap (seal_perm_sentry pc_p) pc_g pc_b pc_e pc_a'
+      }}}.
+  Proof.
+    iIntros (Hinstr Hvpc Hpca' ϕ) "(>HPC & >Hpc_a & >Hcra) Hφ".
+    iApply wp_lift_atomic_base_step_no_fork; auto.
+    iIntros (σ1 ns l1 l2 nt) "[ [Hr0 Hsr] Hm ] /=". destruct σ1 as [ [r0 sr] m]; cbn.
+    iDestruct (@gen_heap_valid with "Hm Hpc_a") as %?; auto.
+    iDestruct (@gen_heap_valid with "Hr0 HPC") as %Hr_PC.
+    iDestruct (@gen_heap_valid with "Hr0 Hcra") as %Hr_cra.
+    iModIntro. iSplitR. by iPureIntro; apply normal_always_base_reducible.
+    iNext. iIntros (e2 σ2 efs Hpstep).
+    apply prim_step_exec_inv in Hpstep as (-> & -> & (c & -> & Hstep)).
+    iIntros "_".
+    iSplitR; auto. eapply step_exec_inv in Hstep; eauto.
+    unfold exec, exec_opt in Hstep.
+    rewrite Hr_PC /= Hpca' /= in Hstep.
+    simplify_pair_eq.
+
+    iMod (@gen_heap_update with "Hr0 Hcra") as "[Hr0 Hcra]".
+    iMod (@gen_heap_update with "Hr0 HPC") as "[Hr0 HPC]".
+    iFrame.
+    iApply "Hφ". by iFrame.
+  Qed.
+
+  Lemma wp_jalr_success_cra E pc_p pc_g pc_b pc_e pc_a pc_a' w wra :
+    decodeInstrW w = Jalr cra →
+    isCorrectPC (WCap pc_p pc_g pc_b pc_e pc_a) →
+    (pc_a + 1)%a = Some pc_a' →
+
+    {{{ ▷ PC ↦ᵣ WCap pc_p pc_g pc_b pc_e pc_a
+        ∗ ▷ pc_a ↦ₐ w
+        ∗ ▷ cra ↦ᵣ wra
+    }}}
+      Instr Executable @ E
+      {{{ RET NextIV;
+          PC ↦ᵣ updatePcPerm wra
+          ∗ pc_a ↦ₐ w
+          ∗ cra ↦ᵣ WCap (seal_perm_sentry pc_p) pc_g pc_b pc_e pc_a'
+      }}}.
+  Proof.
+    iIntros (Hinstr Hvpc Hpca' ϕ) "(>HPC & >Hpc_a & >Hcra) Hφ".
+    iApply wp_lift_atomic_base_step_no_fork; auto.
+    iIntros (σ1 ns l1 l2 nt) "[ [Hr0 Hsr] Hm ] /=". destruct σ1 as [ [r0 sr] m]; cbn.
+    iDestruct (@gen_heap_valid with "Hm Hpc_a") as %?; auto.
+    iDestruct (@gen_heap_valid with "Hr0 HPC") as %Hr_PC.
+    iDestruct (@gen_heap_valid with "Hr0 Hcra") as %Hr_cra.
+    iModIntro. iSplitR. by iPureIntro; apply normal_always_base_reducible.
+    iNext. iIntros (e2 σ2 efs Hpstep).
+    apply prim_step_exec_inv in Hpstep as (-> & -> & (c & -> & Hstep)).
+    iIntros "_".
+    iSplitR; auto. eapply step_exec_inv in Hstep; eauto.
+    unfold exec, exec_opt in Hstep.
+    rewrite Hr_PC /= Hr_cra /= Hpca' /= in Hstep.
+    simplify_pair_eq.
+
+    iMod (@gen_heap_update with "Hr0 Hcra") as "[Hr0 Hcra]".
+    iMod (@gen_heap_update with "Hr0 HPC") as "[Hr0 HPC]".
+    iFrame.
+    iApply "Hφ". by iFrame.
+  Qed.
+
+End cap_lang_rules.
